bringing this stuff in

coq/FwOF/FwOFRelation.v
@@ -3,7 +3,10 @@ Set Implicit Arguments.
 Require Import Coq.Lists.List.
 Require Import Coq.Classes.Equivalence.
 Require Import Coq.Structures.Equalities.
+Require Import Coq.Classes.Morphisms.
+Require Import Coq.Setoids.Setoid.
 Require Import Common.Types.
+Require Import Common.Bisimulation.
 Require Import Bag.Bag.
 Require Import FwOF.FwOF.
 
@@ -11,28 +14,17 @@ Local Open Scope list_scope.
 Local Open Scope equiv_scope.
 Local Open Scope bag_scope.
 
-
 Module Make (Import Atoms : ATOMS).
 
   Module Concrete := ConcreteSemantics (Atoms).
   Import Concrete.
 
-  Definition abst_state := Bag.Bag (switchId * portId * packet).
-  Axiom abst_func : switchId -> portId -> packet -> list (portId * packet).
   Axiom topo : switchId -> portId -> option (switchId * portId).
 
   Definition affixSwitch (sw : switchId) (ptpk : portId * packet) :=
     match ptpk with
       | (pt,pk) => (sw,pt,pk)
     end.
-  
-  Inductive abstractStep : abst_state -> option observation -> abst_state -> 
-    Prop := 
-  | AbstractStep : forall sw pt pk lps,
-    abstractStep
-      ({| (sw,pt,pk) |} <+> lps)
-      (Some (sw,pt,pk))
-      (Bag.from_list (map (affixSwitch sw) (abst_func sw pt pk)) <+> lps).
 
   Definition transfer (sw : switchId) (ptpk : portId * packet) :=
     match ptpk with
@@ -59,10 +51,50 @@ Module Make (Import Atoms : ATOMS).
       | _ => {| |}
     end.
 
+  Definition abst_state := Bag.Bag (switchId * portId * packet).
+
+  Axiom abst_func : switchId -> portId -> packet -> list (portId * packet).
+
+  Definition flow_table_safe (sw : switchId) (tbl : flowTable) : Prop :=
+    forall pt pk forwardedPkts packetIns,
+      process_packet tbl pt pk = (forwardedPkts, packetIns) ->
+      bag_unions (map (transfer sw) forwardedPkts) <+>
+      bag_unions (map (select_packet_in sw) (map (PacketIn pt) packetIns)) ===
+      bag_unions (map (transfer sw) (abst_func sw pt pk)).
+
+  Definition state_switches (st : state) := 
+    match st with
+      | (switches, _, _, _) => switches
+    end.
+
+  Record concreteState := ConcreteState {
+    concreteState_state : state;
+    concreteState_flowTableSafety :
+      forall (sw : switch), 
+        In sw (state_switches concreteState_state) -> 
+        flow_table_safe (switch_swichId sw) (switch_flowTable sw)
+  }.
+
+  Definition concreteStep (st : concreteState) (obs : option observation)
+    (st0 : concreteState) :=
+    step (concreteState_state st) obs (concreteState_state st0).
+
+  Inductive abstractStep : abst_state -> option observation -> abst_state -> 
+    Prop := 
+  | AbstractStepEquiv : forall st st',
+      st === st' ->
+      abstractStep st None st'
+  | AbstractStep : forall sw pt pk lps,
+    abstractStep
+      ({| (sw,pt,pk) |} <+> lps)
+      (Some (sw,pt,pk))
+      (bag_unions (map (transfer sw) (abst_func sw pt pk)) <+> lps).
+
+
   Definition relate_switch (sw : switch) : abst_state :=
     match sw with
       | Switch swId _ tbl inp outp ctrlm switchm =>
-        Bag.map (affixSwitch swId) inp <+>
+        Bag.from_list (map (affixSwitch swId) (Bag.to_list inp)) <+>
         bag_unions (map (transfer swId) (Bag.to_list outp)) <+>
         bag_unions (map (select_packet_out swId) (Bag.to_list ctrlm)) <+>
         bag_unions (map (select_packet_in swId) (Bag.to_list switchm))
@@ -92,9 +124,128 @@ Module Make (Import Atoms : ATOMS).
         relate_controller ctrl
     end.
         
-  Definition bisim_relation (st : state) (ast : abst_state) : Prop :=
-    ast === (relate st).
+  Definition bisim_relation : relation concreteState abst_state :=
+    fun (st : concreteState) (ast : abst_state) => 
+      ast === (relate (concreteState_state st)).
 
+  Section BagAxioms.
+
+    Import Bag.
+
+    Axiom bag_unions_app : forall (A : Type) (E : Eq A)
+      (lst lst0 : list (Bag.Bag A)),
+      bag_unions (lst ++ lst0) === union (bag_unions lst) (bag_unions lst0).
+
+    Axiom bag_unions_cons : forall (A : Type) (E : Eq A)
+      (elt : Bag.Bag A)
+      (lst : list (Bag.Bag A)),
+      bag_unions (elt :: lst) === union elt (bag_unions lst).
+
+    Axiom bag_map_union : forall {A B : Type} {EA : Eq A} {EB : Eq B}
+      (f : A -> B) (bag1 bag2 : Bag.Bag A),
+      (from_list (List.map f (to_list (union bag1 bag2)))) ===
+      (union (from_list (List.map f (to_list bag1))) 
+             (from_list (List.map f (to_list bag2)))).
+
+    Axiom bag_from_list_singleton : forall (A : Type) (E : Eq A)
+      (elt : A),
+      from_list [elt] = singleton elt.
+    
+    Axiom bag_unions_unlist : forall (A B : Type) (EA : Eq A) (EB : Eq B)
+      (f : A -> Bag.Bag B) (lst : list A) (bag : Bag A),
+      bag_unions (List.map f (to_list (from_list lst <+> bag))) = 
+      bag_unions (List.map f lst) <+> 
+      bag_unions (List.map f (to_list bag)).
+
+    Axiom bag_union_red_1 : forall (A : Type) (E : Eq A)
+      (b b0 b1 : Bag A),
+      b <+> b0 === b <+> b1 <-> b0 === b1.
+
+  End BagAxioms.
+
+
+  Theorem weak_sim_1 :
+    weak_simulation concreteStep abstractStep bisim_relation.
+  Proof with auto with datatypes.
+    unfold weak_simulation.
+    intros.
+    split.
+    intros.
+    unfold bisim_relation in H.
+    unfold concreteStep in H0.
+    destruct s. destruct s'. simpl in *.
+    inversion H0; subst.
+    inversion H1; subst.
+    simpl in H.
+    rewrite -> map_app in H.
+    simpl in H.
+    rewrite -> bag_unions_app in H.
+    rewrite -> bag_unions_cons in H.
+    rewrite -> bag_map_union in H.
+    rewrite -> Bag.to_list_singleton in H.
+    simpl in H.
+    repeat rewrite -> Bag.union_assoc in H.
+    rewrite -> Bag.union_comm in H.
+    rewrite -> Bag.union_assoc in H.
+    rewrite -> bag_from_list_singleton in H.
+    match goal with
+      | [ H : t === ?t0 <+> ?t1 |- _ ] => remember t1
+    end.
+    remember(bag_unions (map (transfer swId) (abst_func swId pt pk)) <+> b) as t'.
+    exists t'.
+    split.
+    Focus 2.
+    apply multistep_tau with (a0 := ({|(swId, pt, pk)|}) <+> b).
+    apply AbstractStepEquiv...
+    apply multistep_obs with
+      (a0 := (bag_unions (map (transfer swId) (abst_func swId pt pk)) <+> b)).
+    apply AbstractStep.
+    subst.
+    apply multistep_nil.
+    (* Showing the states are bisimilar *)
+    unfold bisim_relation.
+    simpl.
+    rewrite -> map_app.
+    rewrite -> bag_unions_app.
+    simpl.
+    clear H0. clear H1.
+    rewrite -> bag_unions_unlist.
+    rewrite -> bag_unions_unlist.
+    subst.
+    repeat rewrite -> Bag.union_assoc.
+    unfold state_switches in *.
+    assert (flow_table_safe swId tbl) as J.
+      refine (concreteState_flowTableSafety1
+        (Switch swId pts tbl inp (Bag.from_list outp' <+> outp) ctrlm
+          (Bag.from_list (map (PacketIn pt) pksToCtrl) <+> switchm)) _)...
+      unfold flow_table_safe in J.
+      pose (J0 := J pt pk outp' pksToCtrl H3).
+      rewrite <- J0.
+    admit. (* gotta bubble sort ... *)
+    admit.
+    admit.
+    admit.
+    
+    (* No observations *)
+    intros.
+
+  Admitted.
+    
+  Theorem weak_sim_2 :
+    weak_simulation abstractStep concreteStep (inverse_relation bisim_relation).
+  Proof with auto.
+
+  Admitted.
+
+
+  Theorem fwof_abst_weak_bisim :
+    weak_bisimulation concreteStep abstractStep bisim_relation.
+  Proof.
+    unfold weak_bisimulation.
+    split.
+    exact weak_sim_1.
+    exact weak_sim_2.
+  Qed.
 
 End Make.    
   
