coq/Common/Bisimulation.v
@@ -1,0 +1,50 @@
+Set Implicit Arguments.
+
+Require Common.Types.
+
+Local Open Scope list_scope.
+
+(** [Coq.Relation.Relation_Definitions.relation] has type [A -> A ->
+    Prop], which is not what we want. *)
+Definition relation (A B : Type) := A -> B -> Prop.
+
+Definition inverse_relation (A B : Type) (R : relation A B) : relation B A :=
+  fun (b : B) (a : A) => R a b.
+
+Definition step (A Ob : Type) := A -> option Ob -> A -> Prop.
+
+Inductive multistep (A Ob : Type) (step : step A Ob)
+  : A -> list Ob -> A -> Prop :=
+  | multistep_nil : forall a, multistep step a nil a
+  | multistep_tau : forall a a0 a1 obs,
+    step a None a0 ->
+    multistep step a0 obs a1 ->
+    multistep step a obs a1
+  | multistep_obs : forall a a0 a1 ob obs,
+    step a (Some ob) a0 ->
+    multistep step a0 obs a1 ->
+    multistep step a (ob :: obs) a1.
+
+Definition weak_simulation
+  (S T Ob : Type)
+  (step_S : step S Ob)
+  (step_T : step T Ob)
+  (R : relation S T) :=
+  forall (s : S) (t : T),
+    R s t  ->
+    (forall (s' : S) (a : Ob), step_S s (Some a) s' ->
+      exists (t' : T), 
+        R s' t' /\
+        multistep step_T t (a :: nil) t') /\
+    (forall (s' : S), step_S s None s' ->
+      exists (t' : T), 
+        R s' t' /\
+        multistep step_T t nil t').
+
+Definition weak_bisimulation
+  (S T A : Type) 
+  (step_S : step S A) 
+  (step_T : step T A)
+  (R : relation S T) :=
+  weak_simulation step_S step_T R /\
+  weak_simulation step_T step_S (inverse_relation R).
